theories/Types.v
@@ -139,6 +139,29 @@ Inductive Unrestricted : TUsage -> Prop :=
 Definition Linear (m : TUsage) : Prop :=
   ~ Unrestricted m.
 
+
+(** A cruft type is either a base type or irrelevant.
+    A cruft type represents a type that can be added
+   through the subtyping rule which may not be used
+   by a term.
+*)
+Definition TTCruft (t : TType) : Prop :=
+  match t with
+  | TTBase _ => True
+  | TTMailbox m => Irrelevant m
+  end.
+
+(** A cruft usage-type is either a base type or the usage is
+    secondClass and the type is cruft
+*)
+Definition TUCruft (t : TUsage) : Prop :=
+  match t with
+  | TUBase _ => True
+  | TUUsage SecondClass ty => TTCruft (TTMailbox ty)
+  | _ => False
+  end.
+
+
 End mailbox_types_classes.
 
 Section mailbox_combinations.
@@ -177,109 +200,4 @@ End mailbox_combinations.
 
 Notation "T ⊞ U ~= V" := (TypeCombination T U V) (at level 80) : types_scope.
 Notation "n1 ▷ⁿ n2 ~= n" := (UsageCombination n1 n2 n) (at level 80) : types_scope.
-Notation "J ▷ K ~= L" := (TypeUsageCombination K J L) (at level 80) : types_scope.
-
-(*
-Section mailbox_types_environment.
-
-Context `{M : IMessage Message}.
-
-(** Type environments are list of usage-annotated types because
-    de Bruijn indices are used to represent variables.
-*)
-(* TODO: Maybe move to own section or file *)
-Definition Env := list TUsage.
-
-(*
-Inductive Member : TUsage -> Env -> Prop :=
-    Z : forall env t, Member t (cons t env)
-  | S : forall env t s, Member t env -> Member t (cons s env).
-*)
-
-Fixpoint lookup (n : nat) (env : Env) : option TUsage :=
-  match n, env with
-  | _, nil => None
-  | 0, (T :: env') => Some T
-  | S n', (_ :: env') => lookup n' env'
-  end.
-
-(*
-Fixpoint lookup {env : Environment} {n : nat} (p : n < length env) : TUsage.
-Proof.
-  induction n.
-  - destruct env eqn:E.
-    + simpl in *; now apply PeanoNat.Nat.nlt_0_r in p.
-    + simpl in *. apply t.
-  - destruct env eqn:E.
-    + simpl in *; now apply PeanoNat.Nat.nlt_0_r in p.
-    + simpl in *. apply IHn. lia.
-Defined.
-
-Fixpoint count {env : Environment} {n : nat} (p : n < length env) : Member (lookup p) env.
-Proof.
-  induction n; destruct env eqn:E; simpl in *.
-  - inversion p.
-  - apply Z.
-  - inversion p.
-  - apply IHn.
-Qed.
-*)
-(** Definition 3.4 of environment subtyping.
-    For now we ignore the premise about variables not being in the domain
-*)
-Inductive EnvironmentSubtype : Env -> Env -> Prop :=
-    EnvSubtypeEmpty : EnvironmentSubtype nil nil
-  | EnvSubtypeUn : forall T env1 env2, Unrestricted T -> EnvironmentSubtype env1 env2 -> EnvironmentSubtype (cons T env1) env2
-  | EnvSubtypeSub : forall T1 T2 env1 env2, Subtype T1 T2 -> EnvironmentSubtype env1 env2 -> EnvironmentSubtype (cons T2 env1) (cons T2 env2).
-
-(** Definition 3.8 of environment combination.
-    For now we ignore the premise about variables not being in the domain
-*)
-Inductive EnvironmentCombination : Env -> Env -> Env -> Prop :=
-    EnvCombEmpty : EnvironmentCombination nil nil nil
-  | EnvCombLeft : forall T env1 env2 env, EnvironmentCombination env1 env2 env -> EnvironmentCombination (cons T env1) env2 (cons T env)
-  | EnvCombRight : forall T env1 env2 env, EnvironmentCombination env1 env2 env -> EnvironmentCombination env1 (cons T env2) (cons T env)
-  | EnvCombBoth : forall T T1 T2 env1 env2 env, EnvironmentCombination env1 env2 env -> T1 ▷ T2 ~= T -> EnvironmentCombination (cons T1 env1) (cons T2 env2) (cons T env).
-
-(** Definition 3.9 of disjoint environment combination.
-    For now we ignore the premise about variables not being in the domain
-*)
-Inductive EnvironmentDisjointCombination : Env -> Env -> Env -> Prop :=
-    EnvDisCombEmpty : EnvironmentDisjointCombination nil nil nil
-  | EnvDisCombLeft : forall T env1 env2 env, EnvironmentDisjointCombination env1 env2 env -> EnvironmentDisjointCombination (cons T env1) env2 (cons T env)
-  | EnvDisCombRight : forall T env1 env2 env, EnvironmentDisjointCombination env1 env2 env -> EnvironmentDisjointCombination env1 (cons T env2) (cons T env)
-  | EnvDisCombBoth : forall T env1 env2 env, EnvironmentDisjointCombination env1 env2 env -> EnvironmentDisjointCombination (cons T env1) (cons T env2) (cons T env).
-
-(** 
-  Definition of splitting an environment into n environments.
-  A list is used to keep track of the environments
-*)
-Inductive EnvironmentDisjointCombinationN : list Env -> Env -> Prop :=
-    EnvDisComb2 : forall env env1 env2,
-      EnvironmentDisjointCombination env1 env2 env ->
-      EnvironmentDisjointCombinationN [env1 ; env2] env
-  | EnvDisCombN : forall env env1 env2 env3 envList,
-      EnvironmentDisjointCombination env1 env2 env3 ->
-      EnvironmentDisjointCombinationN (env3 :: envList) env ->
-      EnvironmentDisjointCombinationN (env1 :: env2 :: envList) env.
-
-Fixpoint returnEnvironment (env : Env) : Env := map returnUsage env.
-Fixpoint secondEnvironment (env : Env) : Env := map secondUsage env.
-
-(** An environment is Base if it only contains base types *)
-Fixpoint BaseEnv (e : Env) : Prop :=
-  match e with
-  | nil => True
-  | (TUBase _ :: env') => BaseEnv env'
-  | _ => False
-  end.
-
-End mailbox_types_environment.
-
-Notation "Env1 ≤ₑ Env2" := (EnvironmentSubtype Env1 Env2) (at level 80) : types_scope.
-Notation "Env1 ▷ₑ Env2 ~= Env" := (EnvironmentCombination Env1 Env2 Env) (at level 80) : types_scope.
-Notation "Env1 +ₑ Env2 ~= Env" := (EnvironmentDisjointCombination Env1 Env2 Env) (at level 80) : types_scope.
-Notation "[ Env1 ]+ₑ ~= Env" := (EnvironmentDisjointCombinationN Env1 Env) (at level 80) : types_scope.
-Notation "⌊ Env ⌋ₑ" := (returnEnvironment Env) : types_scope.
-Notation "⌈ Env ⌉ₑ" := (secondEnvironment Env) : types_scope.
-*)
+Notation "J ▷ K ~= L" := (TypeUsageCombination J K L) (at level 80) : types_scope.
